Split TypeChecker and Environment Checker, move auxilliary lemmas to their right place

pcuic/theories/PCUICAstUtils.v
@@ -790,6 +790,19 @@ Proof.
   reflexivity.
 Qed.
 
+Lemma destArity_mkApps_None ctx t l :
+  destArity ctx t = None -> destArity ctx (mkApps t l) = None.
+Proof.
+  induction l in t |- *. trivial.
+  intros H. cbn. apply IHl. reflexivity.
+Qed.
+
+Lemma destArity_mkApps_Ind ctx ind u l :
+  destArity ctx (mkApps (tInd ind u) l) = None.
+Proof.
+  apply destArity_mkApps_None. reflexivity.
+Qed.
+
 (* Helper for nested recursive functions on well-typed terms *)
 
 Section MapInP.
@@ -829,3 +842,47 @@ Proof.
   induction l; simpl; auto.
 Qed.
 Hint Rewrite @map_InP_length : len.
+
+(** Views *)
+
+Definition isSort T :=
+  match T with
+  | tSort u => true
+  | _ => false
+  end.
+
+Inductive view_sort : term -> Type :=
+| view_sort_sort s : view_sort (tSort s)
+| view_sort_other t : ~ isSort t -> view_sort t.
+
+Equations view_sortc (t : term) : view_sort t :=
+  view_sortc (tSort s) := view_sort_sort s;
+  view_sortc t := view_sort_other t _.
+
+Fixpoint isProd t :=
+  match t with
+  | tProd na A B => true
+  | _ => false
+  end.
+
+Inductive view_prod : term -> Type :=
+| view_prod_prod na A b : view_prod (tProd na A b)
+| view_prod_other t : ~ isProd t -> view_prod t.
+
+Equations view_prodc (t : term) : view_prod t :=
+  view_prodc (tProd na A b) := view_prod_prod na A b;
+  view_prodc t := view_prod_other t _.
+
+Definition isInd (t : term) : bool :=
+  match t with
+  | tInd _ _ => true
+  | _ => false
+  end.
+
+Inductive view_ind : term -> Type :=
+| view_ind_tInd ind u : view_ind (tInd ind u)
+| view_ind_other t : negb (isInd t) -> view_ind t.
+
+Equations view_indc (t : term) : view_ind t :=
+  view_indc (tInd ind u) => view_ind_tInd ind u;
+  view_indc t => view_ind_other t _.
