safechecker/theories/PCUICErrors.v
@@ -1,0 +1,269 @@
+
+(* Distributed under the terms of the MIT license. *)
+From MetaCoq.Template Require Import config utils uGraph.
+From MetaCoq.PCUIC Require Import PCUICAst PCUICAstUtils PCUICPretty.
+From Equations Require Import Equations.
+Require Import ssreflect ssrbool.
+
+Local Set Keyed Unification.
+Set Equations Transparent.
+
+Inductive ConversionError :=
+| NotFoundConstants (c1 c2 : kername)
+
+| NotFoundConstant (c : kername)
+
+| LambdaNotConvertibleTypes
+    (Γ1 : context) (na : aname) (A1 t1 : term)
+    (Γ2 : context) (na' : aname) (A2 t2 : term)
+    (e : ConversionError)
+
+| LambdaNotConvertibleAnn
+    (Γ1 : context) (na : aname) (A1 t1 : term)
+    (Γ2 : context) (na' : aname) (A2 t2 : term)
+
+| ProdNotConvertibleDomains
+    (Γ1 : context) (na : aname) (A1 B1 : term)
+    (Γ2 : context) (na' : aname) (A2 B2 : term)
+    (e : ConversionError)
+
+| ProdNotConvertibleAnn
+    (Γ1 : context) (na : aname) (A1 B1 : term)
+    (Γ2 : context) (na' : aname) (A2 B2 : term)
+
+| CaseOnDifferentInd
+    (Γ1 : context)
+    (ind : inductive) (par : nat) (p c : term) (brs : list (nat × term))
+    (Γ2 : context)
+    (ind' : inductive) (par' : nat) (p' c' : term) (brs' : list (nat × term))
+
+| CaseBranchNumMismatch
+    (ind : inductive) (par : nat)
+    (Γ : context) (p c : term) (brs1 : list (nat × term))
+    (m : nat) (br : term) (brs2 : list (nat × term))
+    (Γ' : context) (p' c' : term) (brs1' : list (nat × term))
+    (m' : nat) (br' : term) (brs2' : list (nat × term))
+
+| DistinctStuckProj
+    (Γ : context) (p : projection) (c : term)
+    (Γ' : context) (p' : projection) (c' : term)
+
+| CannotUnfoldFix
+    (Γ : context) (mfix : mfixpoint term) (idx : nat)
+    (Γ' : context) (mfix' : mfixpoint term) (idx' : nat)
+
+| FixRargMismatch (idx : nat)
+    (Γ : context) (u : def term) (mfix1 mfix2 : mfixpoint term)
+    (Γ' : context) (v : def term) (mfix1' mfix2' : mfixpoint term)
+
+| FixMfixMismatch (idx : nat)
+    (Γ : context) (mfix : mfixpoint term)
+    (Γ' : context) (mfix' : mfixpoint term)
+
+| DistinctCoFix
+    (Γ : context) (mfix : mfixpoint term) (idx : nat)
+    (Γ' : context) (mfix' : mfixpoint term) (idx' : nat)
+
+| CoFixRargMismatch (idx : nat)
+    (Γ : context) (u : def term) (mfix1 mfix2 : mfixpoint term)
+    (Γ' : context) (v : def term) (mfix1' mfix2' : mfixpoint term)
+
+| CoFixMfixMismatch (idx : nat)
+    (Γ : context) (mfix : mfixpoint term)
+    (Γ' : context) (mfix' : mfixpoint term)
+
+| StackHeadError
+    (leq : conv_pb)
+    (Γ1 : context)
+    (t1 : term) (args1 : list term) (u1 : term) (l1 : list term)
+    (Γ2 : context)
+    (t2 : term) (u2 : term) (l2 : list term)
+    (e : ConversionError)
+
+| StackTailError (leq : conv_pb)
+    (Γ1 : context)
+    (t1 : term) (args1 : list term) (u1 : term) (l1 : list term)
+    (Γ2 : context)
+    (t2 : term) (u2 : term) (l2 : list term)
+    (e : ConversionError)
+
+| StackMismatch
+    (Γ1 : context) (t1 : term) (args1 l1 : list term)
+    (Γ2 : context) (t2 : term) (l2 : list term)
+
+| HeadMismatch
+    (leq : conv_pb)
+    (Γ1 : context) (t1 : term)
+    (Γ2 : context) (t2 : term).
+
+Inductive type_error :=
+| UnboundRel (n : nat)
+| UnboundVar (id : string)
+| UnboundEvar (ev : nat)
+| UndeclaredConstant (c : kername)
+| UndeclaredInductive (c : inductive)
+| UndeclaredConstructor (c : inductive) (i : nat)
+| NotCumulSmaller (G : universes_graph) (Γ : context) (t u t' u' : term) (e : ConversionError)
+| NotConvertible (G : universes_graph) (Γ : context) (t u : term)
+| NotASort (t : term)
+| NotAProduct (t t' : term)
+| NotAnInductive (t : term)
+| NotAnArity (t : term)
+| IllFormedFix (m : mfixpoint term) (i : nat)
+| UnsatisfiedConstraints (c : ConstraintSet.t)
+| Msg (s : string).
+
+Definition print_level := string_of_level.
+
+Definition string_of_Z z :=
+  if (z <=? 0)%Z then "-" ^ string_of_nat (Z.to_nat (- z)) else string_of_nat (Z.to_nat z).
+
+Definition print_edge '(l1, n, l2)
+  := "(" ^ print_level l1 ^ ", " ^ string_of_Z n ^ ", "
+         ^ print_level l2 ^ ")".
+
+Definition print_universes_graph (G : universes_graph) :=
+  let levels := LevelSet.elements G.1.1 in
+  let edges := wGraph.EdgeSet.elements G.1.2 in
+  string_of_list print_level levels
+  ^ "\n" ^ string_of_list print_edge edges.
+
+Definition string_of_conv_pb (c : conv_pb) : string :=
+  match c with
+  | Conv => "conversion"
+  | Cumul => "cumulativity"
+  end.
+
+Definition print_term Σ Γ t :=
+  print_term Σ Γ true false t.
+
+Fixpoint string_of_conv_error Σ (e : ConversionError) : string :=
+  match e with
+  | NotFoundConstants c1 c2 =>
+      "Both constants " ^ string_of_kername c1 ^ " and " ^ string_of_kername c2 ^
+      " are not found in the environment."
+  | NotFoundConstant c =>
+      "Constant " ^ string_of_kername c ^
+      " common in both terms is not found in the environment."
+  | LambdaNotConvertibleAnn Γ1 na A1 t1 Γ2 na' A2 t2 =>
+      "When comparing\n" ^ print_term Σ Γ1 (tLambda na A1 t1) ^
+      "\nand\n" ^ print_term Σ Γ2 (tLambda na' A2 t2) ^
+      "\nbinding annotations are not convertible\n"
+  | LambdaNotConvertibleTypes Γ1 na A1 t1 Γ2 na' A2 t2 e =>
+      "When comparing\n" ^ print_term Σ Γ1 (tLambda na A1 t1) ^
+      "\nand\n" ^ print_term Σ Γ2 (tLambda na' A2 t2) ^
+      "\ntypes are not convertible:\n" ^
+      string_of_conv_error Σ e
+  | ProdNotConvertibleAnn Γ1 na A1 B1 Γ2 na' A2 B2 =>
+      "When comparing\n" ^ print_term Σ Γ1 (tProd na A1 B1) ^
+      "\nand\n" ^ print_term Σ Γ2 (tProd na' A2 B2) ^
+      "\nbinding annotations are not convertible:\n"
+  | ProdNotConvertibleDomains Γ1 na A1 B1 Γ2 na' A2 B2 e =>
+      "When comparing\n" ^ print_term Σ Γ1 (tProd na A1 B1) ^
+      "\nand\n" ^ print_term Σ Γ2 (tProd na' A2 B2) ^
+      "\ndomains are not convertible:\n" ^
+      string_of_conv_error Σ e
+  | CaseOnDifferentInd Γ ind par p c brs Γ' ind' par' p' c' brs' =>
+      "The two stuck pattern-matching\n" ^
+      print_term Σ Γ (tCase (ind, par) p c brs) ^
+      "\nand\n" ^ print_term Σ Γ' (tCase (ind', par') p' c' brs') ^
+      "\nare done on distinct inductive types."
+  | CaseBranchNumMismatch
+      ind par Γ p c brs1 m br brs2 Γ' p' c' brs1' m' br' brs2' =>
+      "The two stuck pattern-matching\n" ^
+      print_term Σ Γ (tCase (ind, par) p c (brs1 ++ (m,br) :: brs2)) ^
+      "\nand\n" ^
+      print_term Σ Γ' (tCase (ind, par) p' c' (brs1' ++ (m',br') :: brs2')) ^
+      "\nhave a mistmatch in the branch number " ^ string_of_nat #|brs1| ^
+      "\nthe number of parameters do not coincide\n" ^
+      print_term Σ Γ br ^
+      "\nhas " ^ string_of_nat m ^ " parameters while\n" ^
+      print_term Σ Γ br' ^
+      "\nhas " ^ string_of_nat m' ^ "."
+  | DistinctStuckProj Γ p c Γ' p' c' =>
+      "The two stuck projections\n" ^
+      print_term Σ Γ (tProj p c) ^
+      "\nand\n" ^
+      print_term Σ Γ' (tProj p' c') ^
+      "\nare syntactically different."
+  | CannotUnfoldFix Γ mfix idx Γ' mfix' idx' =>
+      "The two fixed-points\n" ^
+      print_term Σ Γ (tFix mfix idx) ^
+      "\nand\n" ^ print_term Σ Γ' (tFix mfix' idx') ^
+      "\ncorrespond to syntactically distinct terms that can't be unfolded."
+  | FixRargMismatch idx Γ u mfix1 mfix2 Γ' v mfix1' mfix2' =>
+      "The two fixed-points\n" ^
+      print_term Σ Γ (tFix (mfix1 ++ u :: mfix2) idx) ^
+      "\nand\n" ^ print_term Σ Γ' (tFix (mfix1' ++ v :: mfix2') idx) ^
+      "\nhave a mismatch in the function number " ^ string_of_nat #|mfix1| ^
+      ": arguments " ^ string_of_nat u.(rarg) ^
+      " and " ^ string_of_nat v.(rarg) ^ "are different."
+  | FixMfixMismatch idx Γ mfix Γ' mfix' =>
+      "The two fixed-points\n" ^
+      print_term Σ Γ (tFix mfix idx) ^
+      "\nand\n" ^
+      print_term Σ Γ' (tFix mfix' idx) ^
+      "\nhave a different number of mutually defined functions."
+  | DistinctCoFix Γ mfix idx Γ' mfix' idx' =>
+      "The two cofixed-points\n" ^
+      print_term Σ Γ (tCoFix mfix idx) ^
+      "\nand\n" ^ print_term Σ Γ' (tCoFix mfix' idx') ^
+      "\ncorrespond to syntactically distinct terms."
+  | CoFixRargMismatch idx Γ u mfix1 mfix2 Γ' v mfix1' mfix2' =>
+      "The two co-fixed-points\n" ^
+      print_term Σ Γ (tCoFix (mfix1 ++ u :: mfix2) idx) ^
+      "\nand\n" ^ print_term Σ Γ' (tCoFix (mfix1' ++ v :: mfix2') idx) ^
+      "\nhave a mismatch in the function number " ^ string_of_nat #|mfix1| ^
+      ": arguments " ^ string_of_nat u.(rarg) ^
+      " and " ^ string_of_nat v.(rarg) ^ "are different."
+  | CoFixMfixMismatch idx Γ mfix Γ' mfix' =>
+      "The two co-fixed-points\n" ^
+      print_term Σ Γ (tCoFix mfix idx) ^
+      "\nand\n" ^
+      print_term Σ Γ' (tCoFix mfix' idx) ^
+      "\nhave a different number of mutually defined functions."
+  | StackHeadError leq Γ1 t1 args1 u1 l1 Γ2 t2 u2 l2 e =>
+      "TODO stackheaderror\n" ^
+      string_of_conv_error Σ e
+  | StackTailError leq Γ1 t1 args1 u1 l1 Γ2 t2 u2 l2 e =>
+      "TODO stacktailerror\n" ^
+      string_of_conv_error Σ e
+  | StackMismatch Γ1 t1 args1 l1 Γ2 t2 l2 =>
+      "Convertible terms\n" ^
+      print_term Σ Γ1 t1 ^
+      "\nand\n" ^ print_term Σ Γ2 t2 ^
+      "are convertible/convertible (TODO) but applied to a different number" ^
+      " of arguments."
+  | HeadMismatch leq Γ1 t1 Γ2 t2 =>
+      "Terms\n" ^
+      print_term Σ Γ1 t1 ^
+      "\nand\n" ^ print_term Σ Γ2 t2 ^
+      "\ndo not have the same head when comparing for " ^
+      string_of_conv_pb leq
+  end.
+
+Definition string_of_type_error Σ (e : type_error) : string :=
+  match e with
+  | UnboundRel n => "Unbound rel " ^ string_of_nat n
+  | UnboundVar id => "Unbound var " ^ id
+  | UnboundEvar ev => "Unbound evar " ^ string_of_nat ev
+  | UndeclaredConstant c => "Undeclared constant " ^ string_of_kername c
+  | UndeclaredInductive c => "Undeclared inductive " ^ string_of_kername (inductive_mind c)
+  | UndeclaredConstructor c i => "Undeclared inductive " ^ string_of_kername (inductive_mind c)
+  | NotCumulSmaller G Γ t u t' u' e => "Terms are not <= for cumulativity:\n" ^
+      print_term Σ Γ t ^ "\nand:\n" ^ print_term Σ Γ u ^
+      "\nafter reduction:\n" ^
+      print_term Σ Γ t' ^ "\nand:\n" ^ print_term Σ Γ u' ^
+      "\nerror:\n" ^ string_of_conv_error Σ e ^
+      "\nin universe graph:\n" ^ print_universes_graph G
+  | NotConvertible G Γ t u => "Terms are not convertible:\n" ^
+      print_term Σ Γ t ^ "\nand:\n" ^ print_term Σ Γ u ^
+      "\nin universe graph:\n" ^ print_universes_graph G
+  | NotASort t => "Not a sort"
+  | NotAProduct t t' => "Not a product"
+  | NotAnArity t => print_term Σ [] t ^ " is not an arity"
+  | NotAnInductive t => "Not an inductive"
+  | IllFormedFix m i => "Ill-formed recursive definition"
+  | UnsatisfiedConstraints c => "Unsatisfied constraints"
+  | Msg s => "Msg: " ^ s
+  end.
