safechecker/theories/PCUICTypeChecker.v
@@ -1,0 +1,932 @@
+(* Distributed under the terms of the MIT license. *)
+From MetaCoq.Template Require Import config utils uGraph.
+From MetaCoq.PCUIC Require Import PCUICAst PCUICAstUtils
+     PCUICLiftSubst PCUICUnivSubst PCUICTyping PCUICNormal PCUICSR
+     PCUICGeneration PCUICReflect PCUICEquality PCUICInversion PCUICValidity
+     PCUICWeakening PCUICPosition PCUICCumulativity PCUICSafeLemmata PCUICSN
+     PCUICPretty PCUICArities PCUICConfluence PCUICSize
+     PCUICContextConversion PCUICConversion PCUICWfUniverses
+     PCUICGlobalEnv
+     (* Used for support lemmas *)
+     PCUICInductives PCUICWfUniverses
+     PCUICContexts PCUICSubstitution PCUICSpine PCUICInductiveInversion
+     PCUICClosed PCUICUnivSubstitution PCUICWeakeningEnv.
+
+From MetaCoq.SafeChecker Require Import PCUICSafeReduce PCUICErrors PCUICEqualityDec
+  PCUICSafeConversion PCUICWfReduction.
+
+From Equations Require Import Equations.
+Require Import ssreflect ssrbool.
+
+Local Set Keyed Unification.
+Set Equations Transparent.
+
+(** It otherwise tries [auto with *], very bad idea. *)
+Ltac Coq.Program.Tactics.program_solve_wf ::= 
+  match goal with 
+  | |- @Wf.well_founded _ _ => auto with subterm wf
+  | |- ?T => match type of T with
+                | Prop => auto
+                end
+  end.
+
+Inductive typing_result (A : Type) :=
+| Checked (a : A)
+| TypeError (t : type_error).
+Global Arguments Checked {A} a.
+Global Arguments TypeError {A} t.
+
+Instance typing_monad : Monad typing_result :=
+  {| ret A a := Checked a ;
+     bind A B m f :=
+       match m with
+       | Checked a => f a
+       | TypeError t => TypeError t
+       end
+  |}.
+
+Instance monad_exc : MonadExc type_error typing_result :=
+  { raise A e := TypeError e;
+    catch A m f :=
+      match m with
+      | Checked a => m
+      | TypeError t => f t
+      end
+  }.
+
+Section Typecheck.
+  Context {cf : checker_flags} {Σ : global_env_ext} (HΣ : ∥ wf Σ ∥)
+          (Hφ : ∥ on_udecl Σ.1 Σ.2 ∥)
+          (G : universes_graph) (HG : is_graph_of_uctx G (global_ext_uctx Σ)).
+
+  (* We get stack overflow on Qed after Equations definitions when this is transparent *)
+  Opaque reduce_stack_full.
+
+  Local Definition HΣ' : ∥ wf_ext Σ ∥.
+  Proof.
+    destruct HΣ, Hφ; now constructor.
+  Defined.
+
+  Definition hnf := reduce_term RedFlags.default Σ HΣ.
+
+  Theorem hnf_sound {Γ t h} : ∥ red (fst Σ) Γ t (hnf Γ t h) ∥.
+  Proof.
+    apply reduce_term_sound.
+  Defined.
+  
+  Theorem hnf_complete {Γ t h} : ∥whnf RedFlags.default Σ Γ (hnf Γ t h)∥.
+  Proof.
+    apply reduce_term_complete.
+  Qed.
+
+  Equations? reduce_to_sort (Γ : context) (t : term) (h : welltyped Σ Γ t)
+    : typing_result (∑ u, ∥ red (fst Σ) Γ t (tSort u) ∥) :=
+    reduce_to_sort Γ t h with view_sortc t := {
+      | view_sort_sort s => ret (s; sq (refl_red _ _ _));
+      | view_sort_other t _ with inspect (hnf Γ t h) :=
+        | exist hnft eq with view_sortc hnft := {
+          | view_sort_sort s => ret (s; _);
+          | view_sort_other t _ => raise (NotASort t)
+        }
+      }.
+  Proof.
+    pose proof (hnf_sound (h:=h)).
+    now rewrite eq.
+  Qed.
+
+  Lemma reduce_to_sort_complete {Γ t wt} e :
+    reduce_to_sort Γ t wt = TypeError e ->
+    (forall s, red Σ Γ t (tSort s) -> False).
+  Proof.
+    funelim (reduce_to_sort Γ t wt); try congruence.
+    intros _ s r.
+    pose proof (@hnf_complete Γ t0 h) as [wh].
+    pose proof (@hnf_sound Γ t0 h) as [r'].
+    destruct HΣ.
+    eapply red_confluence in r as (?&r1&r2); eauto.
+    apply invert_red_sort in r2 as ->.
+    eapply whnf_red_inv in r1; eauto.
+    depelim r1.
+    clear Heq.
+    rewrite H in n0.
+    now cbn in n0.
+  Qed.
+
+  Equations? reduce_to_prod (Γ : context) (t : term) (h : welltyped Σ Γ t)
+    : typing_result (∑ na a b, ∥ red (fst Σ) Γ t (tProd na a b) ∥) :=
+    reduce_to_prod Γ t h with view_prodc t := {
+      | view_prod_prod na a b => ret (na; a; b; sq (refl_red _ _ _));
+      | view_prod_other t _ with inspect (hnf Γ t h) :=
+        | exist hnft eq with view_prodc hnft := {
+          | view_prod_prod na a b => ret (na; a; b; _);
+          | view_prod_other t' _ => raise (NotAProduct t t')
+        }
+      }.
+  Proof.
+    pose proof (hnf_sound (h:=h)).
+    now rewrite eq.
+  Qed.
+
+  Lemma reduce_to_prod_complete {Γ t wt} e :
+    reduce_to_prod Γ t wt = TypeError e ->
+    (forall na a b, red Σ Γ t (tProd na a b) -> False).
+  Proof.
+    funelim (reduce_to_prod Γ t wt); try congruence.
+    intros _ na a b r.
+    pose proof (@hnf_complete Γ t0 h) as [wh].
+    pose proof (@hnf_sound Γ t0 h) as [r'].
+    destruct HΣ.
+    eapply red_confluence in r as (?&r1&r2); eauto.
+    apply invert_red_prod in r2 as (?&?&(->&?)&?); auto.
+    eapply whnf_red_inv in r1; auto.
+    depelim r1.
+    clear Heq.
+    rewrite H in n0.
+    now cbn in n0.
+  Qed.
+
+  Equations? reduce_to_ind (Γ : context) (t : term) (h : welltyped Σ Γ t)
+    : typing_result (∑ i u l, ∥ red (fst Σ) Γ t (mkApps (tInd i u) l) ∥) :=
+    reduce_to_ind Γ t h with inspect (decompose_app t) := {
+      | exist (thd, args) eq_decomp with view_indc thd := {
+        | view_ind_tInd i u => ret (i; u; args; sq _);
+        | view_ind_other t _ with inspect (reduce_stack RedFlags.default Σ HΣ Γ t Empty h) := {
+          | exist (hnft, π) eq with view_indc hnft := {
+            | view_ind_tInd i u with inspect (decompose_stack π) := {
+              | exist (l, _) eq_decomp => ret (i; u; l; _)
+              };
+            | view_ind_other _ _ => raise (NotAnInductive t)
+            }
+          }
+        }
+      }.
+  Proof.
+    - assert (X : mkApps (tInd i u) args = t); [|rewrite X; apply refl_red].
+      etransitivity. 2: symmetry; eapply mkApps_decompose_app.
+      now rewrite <- eq_decomp.
+    - pose proof (reduce_stack_sound RedFlags.default Σ HΣ _ _ Empty h).
+      rewrite <- eq in H.
+      cbn in *.
+      assert (π = appstack l ε) as ->.
+      2: { now rewrite zipc_appstack in H. }
+      unfold reduce_stack in eq.
+      destruct reduce_stack_full as (?&_&stack_val&?).
+      subst x.
+      unfold Pr in stack_val.
+      cbn in *.
+      assert (decomp: decompose_stack π = ((decompose_stack π).1, ε)).
+      { rewrite stack_val.
+        now destruct decompose_stack. }
+      apply decompose_stack_eq in decomp as ->.
+      now rewrite <- eq_decomp0.
+  Qed.
+
+  Lemma reduce_to_ind_complete Γ ty wat e :
+    reduce_to_ind Γ ty wat = TypeError e ->
+    forall ind u args,
+      red Σ Γ ty (mkApps (tInd ind u) args) ->
+      False.
+  Proof.
+    funelim (reduce_to_ind Γ ty wat); try congruence.
+    intros _ ind u args r.
+    pose proof (reduce_stack_whnf RedFlags.default Σ HΣ Γ t ε h) as wh.
+    unfold reduce_stack in *.
+    destruct reduce_stack_full as ((hd&π)&r'&stack_valid&(notapp&_)).
+    destruct wh as [wh].
+    apply Req_red in r' as [r'].
+    unfold Pr in stack_valid.
+    cbn in *.
+    destruct HΣ.
+    eapply red_confluence in r as (?&r1&r2); [|eassumption|exact r'].
+    assert (exists args, π = appstack args ε) as (?&->).
+    { exists ((decompose_stack π).1).
+      assert (decomp: decompose_stack π = ((decompose_stack π).1, ε)).
+      { now rewrite stack_valid; destruct decompose_stack. }
+      now apply decompose_stack_eq in decomp. }
+
+    unfold zipp in wh.
+    rewrite stack_context_appstack decompose_stack_appstack in wh.
+    rewrite zipc_appstack in r1.
+    cbn in *.
+    rewrite app_nil_r in wh.
+    apply red_mkApps_tInd in r2 as (?&->&?); auto.
+    eapply whnf_red_inv in r1; eauto.
+    apply whnf_red_mkApps_inv in r1 as (?&?); auto.
+    depelim w.
+    noconf e0.
+    discriminate i0.
+  Qed.
+
+  Definition isconv Γ := isconv_term Σ HΣ Hφ G HG Γ Conv.
+  Definition iscumul Γ := isconv_term Σ HΣ Hφ G HG Γ Cumul.
+  
+  Program Definition convert Γ t u
+          (ht : welltyped Σ Γ t) (hu : welltyped Σ Γ u)
+    : typing_result (∥ Σ ;;; Γ |- t = u ∥) :=
+    match eqb_term Σ G t u with true => ret _ | false =>
+    match isconv Γ t ht u hu with
+    | ConvSuccess => ret _
+    | ConvError e => (* fallback *)  (* nico *)
+      let t' := hnf Γ t ht in
+      let u' := hnf Γ u hu in
+      (* match leq_term (snd Σ) t' u' with true => ret _ | false => *)
+      raise (NotCumulSmaller G Γ t u t' u' e)
+      (* end *)
+    end end.
+  Next Obligation.
+    symmetry in Heq_anonymous; eapply eqb_term_spec in Heq_anonymous; tea.
+    constructor. now constructor.
+  Qed.
+  Next Obligation.
+    symmetry in Heq_anonymous; apply isconv_term_sound in Heq_anonymous.
+    assumption.
+  Qed.
+
+  Program Definition convert_leq Γ t u
+          (ht : welltyped Σ Γ t) (hu : welltyped Σ Γ u)
+    : typing_result (∥ Σ ;;; Γ |- t <= u ∥) :=
+    match leqb_term Σ G t u with true => ret _ | false =>
+    match iscumul Γ t ht u hu with
+    | ConvSuccess => ret _
+    | ConvError e => (* fallback *)  (* nico *)
+      let t' := hnf Γ t ht in
+      let u' := hnf Γ u hu in
+      (* match leq_term (snd Σ) t' u' with true => ret _ | false => *)
+      raise (NotCumulSmaller G Γ t u t' u' e)
+      (* end *)
+    end end.
+  Next Obligation.
+    symmetry in Heq_anonymous; eapply leqb_term_spec in Heq_anonymous; tea.
+    constructor. now constructor.
+  Qed.
+  Next Obligation.
+    symmetry in Heq_anonymous; apply isconv_term_sound in Heq_anonymous.
+    assumption.
+  Qed.
+
+  Section InferAux.
+    Variable (infer : forall Γ (HΓ : ∥ wf_local Σ Γ ∥) (t : term),
+                 typing_result ({ A : term & ∥ Σ ;;; Γ |- t : A ∥ })).
+
+    Program Definition infer_type Γ HΓ t
+      : typing_result ({u : Universe.t & ∥ Σ ;;; Γ |- t : tSort u ∥}) :=
+      tx <- infer Γ HΓ t ;;
+      u <- reduce_to_sort Γ tx.π1 _ ;;
+      ret (u.π1; _).
+    Next Obligation.
+      eapply validity_wf; eassumption.
+    Defined.
+    Next Obligation.
+      destruct HΣ, HΓ, X, X0.
+      now constructor; eapply type_reduction.
+    Defined.
+
+    Program Definition infer_cumul Γ HΓ t A (hA : ∥ isType Σ Γ A ∥)
+      : typing_result (∥ Σ ;;; Γ |- t : A ∥) :=
+      A' <- infer Γ HΓ t ;;
+      X <- convert_leq Γ A'.π1 A _ _ ;;
+      ret _.
+    Next Obligation. now eapply validity_wf. Qed.
+    Next Obligation. destruct hA; now apply wat_welltyped. Qed.
+    Next Obligation.
+      destruct HΣ, HΓ, hA, X, X0. constructor. eapply type_Cumul'; eassumption.
+    Qed.
+  End InferAux.
+
+
+  Program Definition lookup_ind_decl ind
+    : typing_result
+        ({decl & {body & declared_inductive (fst Σ) decl ind body}}) :=
+    match lookup_env (fst Σ) ind.(inductive_mind) with
+    | Some (InductiveDecl decl) =>
+      match nth_error decl.(ind_bodies) ind.(inductive_ind) with
+      | Some body => ret (decl; body; _)
+      | None => raise (UndeclaredInductive ind)
+      end
+    | _ => raise (UndeclaredInductive ind)
+    end.
+  Next Obligation.
+    split.
+    - symmetry in Heq_anonymous0.
+      etransitivity. eassumption. reflexivity.
+    - now symmetry.
+  Defined.
+
+  Program Definition check_consistent_instance uctx u
+    : typing_result (consistent_instance_ext Σ uctx u)
+    := match uctx with
+       | Monomorphic_ctx _ =>
+         check_eq_nat #|u| 0 (Msg "monomorphic instance should be of length 0")
+       | Polymorphic_ctx (inst, cstrs) =>
+         let '(inst, cstrs) := AUContext.repr (inst, cstrs) in
+         check_eq_true (forallb (fun l => LevelSet.mem l (uGraph.wGraph.V G)) u)
+                       (Msg "instance does not have the right length") ;;
+         (* check_eq_true (forallb (fun l => LevelSet.mem l lvs) u) ;; *)
+         X <- check_eq_nat #|u| #|inst|
+                          (Msg "instance does not have the right length");;
+         match check_constraints G (subst_instance_cstrs u cstrs) with
+         | true => ret (conj _ _)
+         | false => raise (Msg "ctrs not satisfiable")
+         end
+         (* #|u| = #|inst| /\ valid_constraints φ (subst_instance_cstrs u cstrs) *)
+       end.
+  Next Obligation.
+    eapply forallb_All in H. eapply All_forallb'; tea.
+    clear -cf HG. intros x; simpl. apply is_graph_of_uctx_levels.
+  Qed.
+  Next Obligation.
+    repeat split.
+    - now rewrite mapi_length in X.
+    - eapply check_constraints_spec; eauto.
+  Qed.
+
+  Obligation Tactic := Program.Tactics.program_simplify ; eauto 2.
+  
+  Program Definition check_is_allowed_elimination (u : Universe.t) (al : allowed_eliminations) :
+    typing_result (is_allowed_elimination Σ u al) :=
+    let o :=
+    match al return option (is_allowed_elimination Σ u al) with
+    | IntoSProp =>
+      match Universe.is_sprop u with
+      | true => Some _
+      | false => None
+      end
+    | IntoPropSProp =>
+      match is_propositional u with
+      | true => Some _
+      | false => None
+      end
+    | IntoSetPropSProp =>
+      match is_propositional u || check_eqb_universe G u Universe.type0 with
+      | true => Some _
+      | false => None
+      end
+    | IntoAny => Some _
+    end in
+    match o with
+    | Some t => Checked t
+    | None => TypeError (Msg "Cannot eliminate over this sort")
+    end.
+  Next Obligation.
+    unfold is_allowed_elimination, is_allowed_elimination0.
+    destruct check_univs; auto.
+    intros val sat.
+    symmetry in Heq_anonymous.
+    apply is_sprop_val with (v := val) in Heq_anonymous.
+    now rewrite Heq_anonymous.
+  Qed.
+  Next Obligation.
+    unfold is_allowed_elimination, is_allowed_elimination0.
+    destruct check_univs; auto.
+    intros val sat.
+    unfold is_propositional in *.
+    destruct Universe.is_prop eqn:prop.
+    - apply is_prop_val with (v := val) in prop; rewrite prop; auto.
+    - destruct Universe.is_sprop eqn:sprop.
+      + apply is_sprop_val with (v := val) in sprop; rewrite sprop; auto.
+      + discriminate.
+  Qed.
+  Next Obligation.
+    unfold is_allowed_elimination, is_allowed_elimination0.
+    destruct check_univs eqn:cu; auto.
+    intros val sat.
+    unfold is_propositional in *.
+    destruct Universe.is_prop eqn:prop.
+    - apply is_prop_val with (v := val) in prop; rewrite prop; auto.
+    - destruct Universe.is_sprop eqn:sprop.
+      + apply is_sprop_val with (v := val) in sprop; rewrite sprop; auto.
+      + destruct check_eqb_universe eqn:check; [|discriminate].
+        eapply check_eqb_universe_spec' in check; eauto.
+        * unfold eq_universe, eq_universe0 in check.
+          rewrite cu in check.
+          specialize (check val sat).
+          now rewrite check.
+        * destruct HΣ, Hφ.
+          now apply wf_ext_global_uctx_invariants.
+        * destruct HΣ, Hφ.
+          now apply global_ext_uctx_consistent.
+  Qed.
+  Next Obligation.
+    unfold is_allowed_elimination, is_allowed_elimination0.
+    destruct check_univs; auto.
+  Qed.
+
+  Program Fixpoint infer (Γ : context) (HΓ : ∥ wf_local Σ Γ ∥) (t : term) {struct t}
+    : typing_result ({ A : term & ∥ Σ ;;; Γ |- t : A ∥ }) :=
+    match t with
+    | tRel n =>
+      match nth_error Γ n with
+      | Some c => ret ((lift0 (S n)) (decl_type c); _)
+      | None   => raise (UnboundRel n)
+      end
+
+    | tVar n  => raise (UnboundVar n)
+    | tEvar ev args => raise (UnboundEvar ev)
+
+    | tSort u =>
+      check_eq_true (wf_universeb Σ u)
+                    (Msg ("Sort contains an undeclared level " ^ string_of_sort u));;
+      ret (tSort (Universe.super u); _)
+
+    | tProd na A B =>
+      s1 <- infer_type infer Γ HΓ A ;;
+      s2 <- infer_type infer (Γ ,, vass na A) _ B ;;
+      ret (tSort (Universe.sort_of_product s1.π1 s2.π1); _)
+
+    | tLambda na A t =>
+      s1 <- infer_type infer Γ HΓ A ;;
+      B <- infer (Γ ,, vass na A) _ t ;;
+      ret (tProd na A B.π1; _)
+
+    | tLetIn n b b_ty b' =>
+      infer_type infer Γ HΓ b_ty ;;
+      infer_cumul infer Γ HΓ b b_ty _ ;;
+      b'_ty <- infer (Γ ,, vdef n b b_ty) _ b' ;;
+      ret (tLetIn n b b_ty b'_ty.π1; _)
+
+    | tApp t u =>
+      ty <- infer Γ HΓ t ;;
+      pi <- reduce_to_prod Γ ty.π1 _ ;;
+      infer_cumul infer Γ HΓ u pi.π2.π1 _ ;;
+      ret (subst10 u pi.π2.π2.π1; _)
+
+    | tConst cst u =>
+      match lookup_env (fst Σ) cst with
+      | Some (ConstantDecl d) =>
+        check_consistent_instance d.(cst_universes) u ;;
+        let ty := subst_instance_constr u d.(cst_type) in
+        ret (ty; _)
+      |  _ => raise (UndeclaredConstant cst)
+      end
+
+    | tInd ind u =>
+      d <- lookup_ind_decl ind ;;
+      check_consistent_instance d.π1.(ind_universes) u ;;
+      let ty := subst_instance_constr u d.π2.π1.(ind_type) in
+      ret (ty; _)
+
+    | tConstruct ind k u =>
+      d <- lookup_ind_decl ind ;;
+      match nth_error d.π2.π1.(ind_ctors) k with
+      | Some cdecl =>
+        check_consistent_instance d.π1.(ind_universes) u ;;
+        ret (type_of_constructor d.π1 cdecl (ind, k) u; _)
+      | None => raise (UndeclaredConstructor ind k)
+      end
+
+    | tCase (ind, par) p c brs =>
+      cty <- infer Γ HΓ c ;;
+      I <- reduce_to_ind Γ cty.π1 _ ;;
+      let '(ind'; I') := I in let '(u; I'') := I' in let '(args; H) := I'' in
+      check_eq_true (eqb ind ind')
+                    (* bad case info *)
+                    (NotConvertible G Γ (tInd ind u) (tInd ind' u)) ;;
+      d <- lookup_ind_decl ind' ;;
+      let '(decl; d') := d in let '(body; HH) := d' in
+      check_coind <- check_eq_true (negb (isCoFinite (ind_finite decl)))
+            (Msg "Case on coinductives disallowed") ;;
+      check_eq_true (ind_npars decl =? par)
+                    (Msg "not the right number of parameters") ;;
+      pty <- infer Γ HΓ p ;;
+      match destArity [] pty.π1 with
+      | None => raise (Msg "the type of the return predicate of a Case is not an arity")
+      | Some (pctx, ps) =>
+        check_is_allowed_elimination ps (ind_kelim body);;
+        let params := firstn par args in
+        match build_case_predicate_type ind decl body params u ps with
+        | None => raise (Msg "failure in build_case_predicate_type")
+        | Some pty' =>
+          (* We could avoid one useless sort comparison by only comparing *)
+          (* the contexts [pctx] and [indctx] (what is done in Coq). *)
+          match iscumul Γ pty.π1 _ pty' _ with
+          | ConvError e => raise (NotCumulSmaller G Γ pty.π1 pty' pty.π1 pty' e)
+          | ConvSuccess =>
+            match map_option_out (build_branches_type ind decl body params u p) with
+            | None => raise (Msg "failure in build_branches_type")
+            | Some btys =>
+              let btyswf : ∥ All (isType Σ Γ ∘ snd) btys ∥ := _ in
+              (fix check_branches (brs btys : list (nat * term))
+                (HH : ∥ All (isType Σ Γ ∘ snd) btys ∥) {struct brs}
+                  : typing_result
+                    (All2 (fun br bty => br.1 = bty.1 /\ ∥ Σ ;;; Γ |- br.2 : bty.2 ∥) brs btys)
+                          := match brs, btys with
+                             | [], [] => ret All2_nil
+                             | (n, t) :: brs , (m, A) :: btys =>
+                               W <- check_dec (Msg "not nat eq")
+                                             (EqDecInstances.nat_eqdec n m) ;;
+                               Z <- infer_cumul infer Γ HΓ t A _ ;;
+                               X <- check_branches brs btys _ ;;
+                               ret (All2_cons (conj _ _) X)
+                             | [], _ :: _
+                             | _ :: _, [] => raise (Msg "wrong number of branches")
+                             end) brs btys btyswf ;;
+                ret (mkApps p (List.skipn par args ++ [c]); _)
+            end
+          end
+        end
+      end
+
+    | tProj (ind, n, k) c =>
+      d <- lookup_ind_decl ind ;;
+      match nth_error d.π2.π1.(ind_projs) k with
+      | Some pdecl =>
+        c_ty <- infer Γ HΓ c ;;
+        I <- reduce_to_ind Γ c_ty.π1 _ ;;
+        let '(ind'; I') := I in let '(u; I'') := I' in let '(args; H) := I'' in
+        check_eq_true (eqb ind ind')
+                      (NotConvertible G Γ (tInd ind u) (tInd ind' u)) ;;
+        check_eq_true (ind_npars d.π1 =? n)
+                      (Msg "not the right number of parameters") ;;
+        let ty := snd pdecl in
+        ret (subst0 (c :: List.rev args) (subst_instance_constr u ty);
+                _)
+      | None => raise (Msg "projection not found")
+      end
+
+    | tFix mfix n =>
+      match nth_error mfix n with
+      | None => raise (IllFormedFix mfix n)
+      | Some decl =>
+        XX <- (fix check_types (mfix : mfixpoint term) {struct mfix}
+              : typing_result (∥ All (fun x => isType Σ Γ (dtype x)) mfix ∥)
+              := match mfix with
+                 | [] => ret (sq All_nil)
+                 | def :: mfix =>
+       (* probably not tail recursive but needed so that next line terminates *)
+                   W <- infer_type infer Γ HΓ (dtype def) ;;
+                   Z <- check_types mfix ;;
+                   ret _
+                 end)
+           mfix ;;
+        YY <- (fix check_bodies (mfix' : mfixpoint term)
+              (XX : ∥ All (fun x => isType Σ Γ (dtype x)) mfix' ∥)
+            {struct mfix'}
+                : typing_result (All (fun d =>
+              ∥ Σ ;;; Γ ,,, fix_context mfix |- dbody d : (lift0 #|fix_context mfix|) (dtype d) ∥
+              /\ isLambda (dbody d) = true) mfix')
+              := match mfix' with
+                 | [] => ret All_nil
+                 | def :: mfix' =>
+                   W1 <- infer_cumul infer (Γ ,,, fix_context mfix) _ (dbody def)
+                                    (lift0 #|fix_context mfix| (dtype def)) _ ;;
+                   W2 <- check_eq_true (isLambda (dbody def))
+                                      (Msg "not a lambda") ;;
+                   Z <- check_bodies mfix' _ ;;
+                   ret (All_cons (conj W1 W2) Z)
+                 end) mfix _ ;;
+        guarded <- check_eq_true (fix_guard mfix) (Msg "Unguarded fixpoint") ;;
+        wffix <- check_eq_true (wf_fixpoint Σ.1 mfix) (Msg "Ill-formed fixpoint: not defined on a mutually inductive family") ;;
+        ret (dtype decl; _)
+      end
+
+    | tCoFix mfix n =>
+      match nth_error mfix n with
+      | None => raise (IllFormedFix mfix n)
+      | Some decl =>
+        XX <-  (fix check_types (mfix : mfixpoint term) {struct mfix}
+        : typing_result (∥ All (fun x => isType Σ Γ (dtype x)) mfix ∥)
+        := match mfix with
+           | [] => ret (sq All_nil)
+           | def :: mfix =>
+            (* probably not tail recursive but needed so that next line terminates *)
+             W <- infer_type infer Γ HΓ (dtype def) ;;
+             Z <- check_types mfix ;;
+             ret _
+           end)
+         mfix ;;
+        YY <- (fix check_bodies (mfix' : mfixpoint term)
+        (XX' : ∥ All (fun x => isType Σ Γ (dtype x)) mfix' ∥)
+        {struct mfix'}
+        : typing_result (All (fun d =>
+            ∥ Σ ;;; Γ ,,, fix_context mfix |- dbody d : (lift0 #|fix_context mfix|) (dtype d) ∥) mfix')
+              := match mfix' with
+                 | [] => ret All_nil
+                 | def :: mfix' =>
+                   W1 <- infer_cumul infer (Γ ,,, fix_context mfix) _ (dbody def)
+                                    (lift0 #|fix_context mfix| (dtype def)) _ ;;
+                   Z <- check_bodies mfix' _ ;;
+                   ret (All_cons W1 Z)
+                 end) mfix _ ;;
+        guarded <- check_eq_true (cofix_guard mfix) (Msg "Unguarded cofixpoint") ;;
+        wfcofix <- check_eq_true (wf_cofixpoint Σ.1 mfix) (Msg "Ill-formed cofixpoint: not producing values in a mutually coinductive family") ;;
+        ret (dtype decl; _)
+      end
+    end.
+
+  (* tRel *)
+  Next Obligation. intros; sq; now econstructor. Defined.
+  (* tSort *)
+  Next Obligation.
+    eapply (elimT wf_universe_reflect) in H.
+    sq; econstructor; tas.
+  Defined.
+  (* tProd *)
+  Next Obligation.
+    (* intros Γ HΓ t na A B Heq_t [s ?];  *)
+      sq; econstructor; cbn; easy. Defined.
+  Next Obligation.
+    (* intros Γ HΓ t na A B Heq_t [s1 ?] [s2 ?]; *)
+    sq; econstructor; eassumption.
+  Defined.
+  (* tLambda *)
+  Next Obligation.
+    (* intros Γ HΓ t0 na A t Heq_t [s ?]; *)
+      sq; econstructor; cbn; easy.
+  Defined.
+  Next Obligation.
+    (* intros Γ HΓ t0 na A t Heq_t [s ?] [B ?]; *)
+      sq; econstructor; eassumption.
+  Defined.
+  (* tLetIn *)
+  Next Obligation.
+    (* intros Γ HΓ t n b b_ty b' Heq_t [? ?]; *)
+      sq. econstructor; eauto.
+  Defined.
+  Next Obligation.
+    (* intros Γ HΓ t n b b_ty b' Heq_t [? ?] H0; *)
+    sq; econstructor; cbn; eauto.
+  Defined.
+  Next Obligation.
+    (* intros Γ HΓ t n b b_ty b' Heq_t [? ?] H0 [? ?]; *)
+    sq; econstructor; eassumption.
+  Defined.
+
+  (* tApp *)
+  Next Obligation. simpl; eauto using validity_wf. Qed.
+  Next Obligation.
+    cbn in *; sq.
+    eapply type_reduction in X1 ; try eassumption.
+    eapply validity_term in X1 ; try assumption. destruct X1 as [s HH].
+    eapply inversion_Prod in HH ; try assumption.
+    destruct HH as [s1 [_ [HH _]]].
+    eexists. eassumption.
+  Defined.
+  Next Obligation.
+    cbn in *; sq; econstructor.
+    2: eassumption.
+    eapply type_reduction; eassumption.
+  Defined.
+
+  (* tConst *)
+  Next Obligation.
+    rename Heq_anonymous into HH.
+    sq; constructor; try assumption.
+    symmetry in HH.
+    etransitivity. eassumption. reflexivity.
+  Defined.
+
+  (* tInd *)
+  Next Obligation.
+    sq; econstructor; eassumption.
+  Defined.
+
+  (* tConstruct *)
+  Next Obligation.
+    sq; econstructor; tea. now split.
+  Defined.
+
+  (* tCase *)
+  Next Obligation. simpl; eauto using validity_wf. Qed.
+  Next Obligation. simpl; eauto using validity_wf. Qed.
+  Next Obligation.
+    destruct X, X9. sq.
+    change (eqb ind I = true) in H0.
+    destruct (eqb_spec ind I) as [e|e]; [destruct e|discriminate].
+    change (eqb (ind_npars d) par = true) in H1.
+    destruct (eqb_spec (ind_npars d) par) as [e|e]; [|discriminate].
+    rename Heq_anonymous into HH. symmetry in HH.
+    simpl in *.
+    eapply type_reduction in t0; eauto. eapply validity in t0; eauto.
+    rewrite <- e in HH.
+    eapply PCUICInductiveInversion.WfArity_build_case_predicate_type in HH; eauto.
+    destruct HH as [[s Hs] ?]. eexists; eauto.
+    eapply validity in t; eauto.
+    generalize (PCUICClosed.destArity_spec [] pty).
+    rewrite -Heq_anonymous0 /=. intros ->.
+    eapply PCUICInductives.isType_it_mkProd_or_LetIn_inv in t; eauto.
+    eapply isType_wf_universes in t. simpl in t.
+    now exact (elimT wf_universe_reflect t). auto.
+  Qed.
+
+  Next Obligation.
+    symmetry in Heq_anonymous2.
+    unfold iscumul in Heq_anonymous2. simpl in Heq_anonymous2.
+    apply isconv_term_sound in Heq_anonymous2.
+    red in Heq_anonymous2.
+    noconf Heq_I''.
+    noconf Heq_I'. noconf Heq_I.
+    noconf Heq_d. noconf Heq_d'.
+    simpl in *; sq.
+    change (eqb ind I = true) in H0.
+    destruct (eqb_spec ind I) as [e|e]; [destruct e|discriminate H0].
+    change (eqb (ind_npars d) par = true) in H1.
+    destruct (eqb_spec (ind_npars d) par) as [e|e]; [|discriminate]; subst.
+    assert (wfΣ : wf_ext Σ) by (split; auto).
+    eapply type_reduction in X9; eauto.
+    have val:= validity_term wfΣ X9.
+    eapply type_Cumul' in X; [| |eassumption].
+    2:{ eapply PCUICInductiveInversion.WfArity_build_case_predicate_type; eauto.
+        eapply validity in X; eauto.
+        generalize (PCUICClosed.destArity_spec [] pty).
+        rewrite -Heq_anonymous0 /=. intros ->.
+        eapply PCUICInductives.isType_it_mkProd_or_LetIn_inv in X; eauto.
+        eapply isType_wf_universes in X. simpl in X.
+        now exact (elimT wf_universe_reflect X). auto. }
+    have [pctx' da] : (∑ pctx', destArity [] pty' =  Some (pctx', ps)).
+    { symmetry in Heq_anonymous1.
+      unshelve eapply (PCUICInductives.build_case_predicate_type_spec (Σ.1, ind_universes d)) in Heq_anonymous1 as [parsubst [_ ->]].
+      eauto. eapply (PCUICWeakeningEnv.on_declared_inductive wfΣ) in HH as [? ?]. eauto.
+      eexists. rewrite !destArity_it_mkProd_or_LetIn; simpl. reflexivity. }
+    eapply PCUICInductiveInversion.build_branches_type_wt. 6:eapply X. all:eauto.
+  Defined.
+
+  Obligation Tactic := simpl; intros.
+
+  Next Obligation.
+    rename Heq_anonymous2 into XX2.
+    symmetry in XX2. simpl in *. eapply isconv_sound in XX2.
+    change (eqb ind ind' = true) in H0.
+    destruct (eqb_spec ind ind') as [e|e]; [destruct e|discriminate H0].
+    change (eqb (ind_npars decl) par = true) in H1.
+    destruct (eqb_spec (ind_npars decl) par) as [e|e]; [|discriminate]; subst.
+    depelim HH.
+    sq. auto. now depelim X.
+  Defined.
+  Next Obligation.
+    sq. now depelim HH.
+  Defined.
+
+  (* The obligation tactic removes a useful let here. *)
+  Obligation Tactic := idtac.
+  Next Obligation.
+    intros. clearbody btyswf. idtac; Program.Tactics.program_simplify.
+    symmetry in Heq_anonymous2.
+    unfold iscumul in Heq_anonymous2. simpl in Heq_anonymous2.
+    apply isconv_term_sound in Heq_anonymous2.
+    noconf Heq_I''. noconf Heq_I'. noconf Heq_I.
+    noconf Heq_d. noconf Heq_d'. simpl in *.
+    assert (∥ All2 (fun x y  => ((fst x = fst y) *
+                              (Σ;;; Γ |- snd x : snd y) * isType Σ Γ y.2)%type) brs btys ∥). {
+      solve_all. simpl in *.
+      destruct btyswf. eapply All2_sq. solve_all. simpl in *; intuition (sq; auto). }
+    clear H3. sq.
+    change (eqb ind I = true) in H0.
+    destruct (eqb_spec ind I) as [e|e]; [destruct e|discriminate H0].
+    change (eqb (ind_npars d) par = true) in H1.
+    destruct (eqb_spec (ind_npars d) par) as [e|e]; [|discriminate]; subst.
+    assert (wfΣ : wf_ext Σ) by (split; auto).
+    eapply type_reduction in X9; eauto.
+    eapply type_Cumul' in X; eauto.
+    2:{ eapply PCUICInductiveInversion.WfArity_build_case_predicate_type; eauto.
+        now eapply validity in X9.
+        eapply validity in X; eauto.
+        generalize (PCUICClosed.destArity_spec [] pty).
+        rewrite -Heq_anonymous0 /=. intros ->.
+        eapply PCUICInductives.isType_it_mkProd_or_LetIn_inv in X; eauto.
+        eapply isType_wf_universes in X. simpl in X.
+        now exact (elimT wf_universe_reflect X). auto. }
+    have [pctx' da] : (∑ pctx', destArity [] pty' =  Some (pctx', ps)).
+    { symmetry in Heq_anonymous1.
+      unshelve eapply (PCUICInductives.build_case_predicate_type_spec (Σ.1, ind_universes d)) in Heq_anonymous1 as [parsubst [_ ->]].
+      eauto. eapply (PCUICWeakeningEnv.on_declared_inductive wfΣ) in HH as [? ?]. eauto.
+      eexists. rewrite !destArity_it_mkProd_or_LetIn; simpl. reflexivity. }
+    eapply type_Case with (pty0:=pty'); tea.
+    - reflexivity.
+    - symmetry; eassumption.
+    - destruct isCoFinite; auto.
+    - symmetry; eauto.
+  Defined.
+
+  Obligation Tactic := Program.Tactics.program_simplify ; eauto 2.
+
+  (* tProj *)
+  Next Obligation. simpl; eauto using validity_wf. Qed.
+  Next Obligation.
+    simpl in *; sq; eapply type_Proj with (pdecl := (i, t0)).
+    - split. eassumption. split. symmetry; eassumption. cbn in *.
+      now apply beq_nat_true.
+    - cbn. destruct (ssrbool.elimT (eqb_spec ind I)); [assumption|].
+      eapply type_reduction; eassumption.
+    - eapply type_reduction in X5; eauto.
+      eapply validity_term in X5; eauto.
+      destruct (ssrbool.elimT (eqb_spec ind I)); auto.
+      unshelve eapply (PCUICInductives.isType_mkApps_Ind _ X7 _) in X5 as [parsubst [argsubst [[sp sp'] cu]]]; eauto.
+      pose proof (PCUICContexts.context_subst_length2 (PCUICSpine.inst_ctx_subst sp)).
+      pose proof (PCUICContexts.context_subst_length2 (PCUICSpine.inst_ctx_subst sp')).
+      autorewrite with len in H, H2.
+      destruct (PCUICWeakeningEnv.on_declared_inductive HΣ X7) eqn:ond.
+      rewrite -o.(onNpars) -H.
+      forward (o0.(onProjections)).
+      intros H'; rewrite H' nth_error_nil // in Heq_anonymous.
+      destruct ind_cshapes as [|cs []]; auto.
+      intros onps.
+      unshelve epose proof (onps.(on_projs_noidx _ _ _ _ _ _)).
+      rewrite ond /= in H2.
+      change (ind_indices o0) with (ind_indices o0) in *.
+      destruct (ind_indices o0) => //.
+      simpl in H2.
+      rewrite List.skipn_length in H2.
+      rewrite List.firstn_length. lia.
+  Qed.
+
+  (* tFix *)
+  Next Obligation. sq. constructor; auto. exists W; auto. Defined.
+  Next Obligation. sq. now eapply PCUICWeakening.All_mfix_wf in XX0. Defined.
+  Next Obligation.
+    sq. cbn in *. depelim XX.
+    destruct i as [s HH].
+    exists s.
+    change (tSort s) with (lift0 #|fix_context mfix| (tSort s)).
+    apply weakening; try assumption.
+    now apply All_mfix_wf.
+  Defined.
+  Next Obligation.
+    clear -XX HΣ. sq.
+    now depelim XX.
+  Qed.
+  Next Obligation.
+    assert (∥ All (fun d => ((Σ;;; Γ ,,, fix_context mfix |- dbody d : (lift0 #|fix_context mfix|) (dtype d)) * (isLambda (dbody d) = true))%type) mfix ∥). {
+      eapply All_sq, All_impl.  exact YY.
+      cbn; intros ? []. sq; now constructor. }
+    sq; econstructor; try eassumption.
+    symmetry; eassumption.
+  Qed.
+
+  (* tCoFix *)
+  Next Obligation. sq. constructor; auto. exists W; auto. Defined.
+  Next Obligation. sq. now eapply PCUICWeakening.All_mfix_wf in XX. Defined.
+  Next Obligation.
+    sq. cbn in *. depelim XX'.
+    destruct i as [s HH].
+    exists s.
+    change (tSort s) with (lift0 #|fix_context mfix| (tSort s)).
+    apply weakening; try assumption.
+    now apply All_mfix_wf.
+  Defined.
+  Next Obligation.
+    clear -XX' HΣ. sq.
+    now depelim XX'.
+  Qed.
+  Next Obligation.
+    assert (∥ All (fun d => ((Σ;;; Γ ,,, fix_context mfix |- dbody d : (lift0 #|fix_context mfix|) (dtype d)))%type) mfix ∥). {
+      eapply All_sq, All_impl.  exact YY.
+      now cbn; intros ? []. }
+    sq; econstructor; try eassumption.
+    symmetry; eassumption.
+  Qed.
+
+  Lemma sq_wfl_nil : ∥ wf_local Σ [] ∥.
+  Proof.
+   repeat constructor.
+  Qed.
+
+  Program Fixpoint check_context Γ : typing_result (∥ wf_local Σ Γ ∥)
+    := match Γ with
+       | [] => ret sq_wfl_nil
+       | {| decl_body := None; decl_type := A |} :: Γ =>
+         HΓ <- check_context Γ ;;
+         XX <- infer_type infer Γ HΓ A ;;
+         ret _
+       | {| decl_body := Some t; decl_type := A |} :: Γ =>
+         HΓ <- check_context Γ ;;
+         XX <- infer_type infer Γ HΓ A ;;
+         XX <- infer_cumul infer Γ HΓ t A _ ;;
+         ret _
+       end.
+  Next Obligation.
+    sq. econstructor; tas. econstructor; eauto.
+  Qed.
+  Next Obligation.
+    sq. econstructor; tea.
+  Qed.
+  Next Obligation.
+    sq. econstructor; tas. econstructor; eauto.
+  Qed.
+
+(* 
+  Program Definition check_isWfArity Γ (HΓ : ∥ wf_local Σ Γ ∥) A
+    : typing_result (∥ isWfArity Σ Γ A ∥) :=
+    match destArity [] A with
+    | None => raise (Msg (print_term Σ Γ A ^ " is not an arity"))
+    | Some (ctx, s) => XX <- check_context (Γ ,,, ctx) ;;
+                      ret _
+    end.
+  Next Obligation.
+    destruct XX. constructor. exists ctx, s.
+    split; auto.
+  Defined. *)
+
+  Program Definition check_isType Γ (HΓ : ∥ wf_local Σ Γ ∥) A
+    : typing_result (∥ isType Σ Γ A ∥) :=
+    s <- infer Γ HΓ A ;;
+    s' <- reduce_to_sort Γ s.π1 _ ;;
+    ret _.
+  Next Obligation. now eapply validity_wf. Defined.
+  Next Obligation. destruct X0. sq. eexists. eapply type_reduction; tea. Defined.
+
+  Program Definition check Γ (HΓ : ∥ wf_local Σ Γ ∥) t A
+    : typing_result (∥ Σ;;; Γ |- t : A ∥) :=
+    check_isType Γ HΓ A ;;
+    infer_cumul infer Γ HΓ t A _.
+
+End Typecheck.
